heap_lang/sugar.v
@@ -2,30 +2,12 @@ Require Export heap_lang.heap_lang heap_lang.lifting.
 Import uPred heap_lang.
 
 (** Define some syntactic sugar. LitTrue and LitFalse are defined in heap_lang.v. *)
-Definition Lam (e : {bind expr}) := Rec e.[ren(+1)].
-Definition Let (e1 : expr) (e2: {bind expr}) := App (Lam e2) e1.
-Definition Seq (e1 e2 : expr) := Let e1 e2.[ren(+1)].
-
-Definition LamV (e : {bind expr}) := RecV e.[ren(+1)].
-
-Definition LetCtx (e2 : {bind expr}) := AppRCtx (LamV e2).
-Definition SeqCtx (e2 : expr) := LetCtx (e2.[ren(+1)]).
-
-(* Prove and "register" compatibility with substitution. *)
-Lemma Lam_subst e s : (Lam e).[s] = Lam e.[up s].
-Proof. by unfold Lam; asimpl. Qed.
-Hint Rewrite Lam_subst : autosubst.
-Global Opaque Lam.
-
-Lemma Let_subst e1 e2 s : (Let e1 e2).[s] = Let e1.[s] e2.[up s].
-Proof. by unfold Let; asimpl. Qed.
-Hint Rewrite Let_subst : autosubst.
-Global Opaque Let.
-
-Lemma Seq_subst e1 e2 s : (Seq e1 e2).[s] = Seq e1.[s] e2.[s].
-Proof. by unfold Seq; asimpl. Qed.
-Hint Rewrite Seq_subst : autosubst.
-Global Opaque Seq.
+Notation Lam x e := (Rec "" x e).
+Notation Let x e1 e2 := (App (Lam x e2) e1).
+Notation Seq e1 e2 := (Let "" e1 e2).
+Notation LamV x e := (RecV "" x e).
+Notation LetCtx x e2 := (AppRCtx (LamV x e2)).
+Notation SeqCtx e2 := (LetCtx "" e2).
 
 Module notations.
   Delimit Scope lang_scope with L.
@@ -36,16 +18,12 @@ Module notations.
   Coercion LitBool : bool >-> base_lit.
   (* No coercion from base_lit to expr. This makes is slightly easier to tell
      apart language and Coq expressions. *)
-  Coercion Loc : loc >-> expr.
-  Coercion LocV : loc >-> val.
+  Coercion Var : string >-> expr.
   Coercion App : expr >-> Funclass.
 
   (** Syntax inspired by Coq/Ocaml. Constructions with higher precedence come
   first. *)
   (* What about Arguments for hoare triples?. *)
-  (* The colons indicate binders. "let" is not consistent here though,
-     thing are only bound in the "in". *)
-  Notation "# n" := (ids (term:=expr) n) (at level 1, format "# n") : lang_scope.
   Notation "! e" := (Load e%L) (at level 10, format "! e") : lang_scope.
   Notation "'ref' e" := (Alloc e%L) (at level 30) : lang_scope.
   Notation "e1 + e2" := (BinOp PlusOp e1%L e2%L)
@@ -57,14 +35,19 @@ Module notations.
   Notation "e1 = e2" := (BinOp EqOp e1%L e2%L) (at level 70) : lang_scope.
   (* The unicode ← is already part of the notation "_ ← _; _" for bind. *)
   Notation "e1 <- e2" := (Store e1%L e2%L) (at level 80) : lang_scope.
-  Notation "e1 ; e2" := (Seq e1%L e2%L)
-    (at level 100, e2 at level 200) : lang_scope.
-  Notation "'let:' e1 'in' e2" := (Let e1%L e2%L)
-    (at level 102, e2 at level 200) : lang_scope.
-  Notation "'λ:' e" := (Lam e%L) (at level 102, e at level 200) : lang_scope.
-  Notation "'rec::' e" := (Rec e%L) (at level 102, e at level 200) : lang_scope.
+  Notation "'rec:' f x := e" := (Rec f x e%L)
+    (at level 102, f at level 1, x at level 1, e at level 200) : lang_scope.
   Notation "'if' e1 'then' e2 'else' e3" := (If e1%L e2%L e3%L)
     (at level 200, e1, e2, e3 at level 200) : lang_scope.
+
+  (* derived notions, in order of declaration *)
+  Notation "λ: x , e" := (Lam x e%L)
+    (at level 102, x at level 1, e at level 200) : lang_scope.
+  (* FIXME: the ones below are not being pretty printed *)
+  Notation "'let:' x := e1 'in' e2" := (Let x e1%L e2%L)
+    (at level 102, x at level 1, e1 at level 1, e2 at level 200) : lang_scope.
+  Notation "e1 ; e2" := (Seq e1%L e2%L)
+    (at level 100, e2 at level 200) : lang_scope.
 End notations.
 
 Section suger.
@@ -73,34 +56,26 @@ Implicit Types P : iProp heap_lang Σ.
 Implicit Types Q : val → iProp heap_lang Σ.
 
 (** Proof rules for the sugar *)
-Lemma wp_lam E ef e v Q :
-  to_val e = Some v → ▷ wp E ef.[e/] Q ⊑ wp E (App (Lam ef) e) Q.
-Proof.
-  intros Hv. rewrite -wp_rec; last eassumption.
-  (* RJ: This pulls in functional extensionality. If that bothers us, we have
-     to talk to the Autosubst guys. *)
-  by asimpl.
-Qed.
+Lemma wp_lam E x ef e v Q :
+  to_val e = Some v → ▷ wp E (subst ef x v) Q ⊑ wp E (App (Lam x ef) e) Q.
+Proof. intros. by rewrite -wp_rec ?subst_empty; eauto. Qed.
 
-Lemma wp_let E e1 e2 Q :
-  wp E e1 (λ v, ▷wp E (e2.[of_val v/]) Q) ⊑ wp E (Let e1 e2) Q.
+Lemma wp_let E x e1 e2 Q :
+  wp E e1 (λ v, ▷ wp E (subst e2 x v) Q) ⊑ wp E (Let x e1 e2) Q.
 Proof.
-  rewrite -(wp_bind [LetCtx e2]). apply wp_mono=>v.
+  rewrite -(wp_bind [LetCtx x e2]). apply wp_mono=>v.
   by rewrite -wp_lam //= to_of_val.
 Qed.
 
-Lemma wp_seq E e1 e2 Q :
-  wp E e1 (λ _, ▷wp E e2 Q) ⊑ wp E (Seq e1 e2) Q.
-Proof.
-  rewrite -wp_let. apply wp_mono=>v. by asimpl.
-Qed.
+Lemma wp_seq E e1 e2 Q : wp E e1 (λ _, ▷wp E e2 Q) ⊑ wp E (Seq e1 e2) Q.
+Proof. rewrite -wp_let. apply wp_mono=>v. by rewrite subst_empty. Qed.
 
 Lemma wp_le E (n1 n2 : nat) P Q :
   (n1 ≤ n2 → P ⊑ ▷ Q (LitV true)) →
   (n1 > n2 → P ⊑ ▷ Q (LitV false)) →
   P ⊑ wp E (BinOp LeOp (Lit n1) (Lit n2)) Q.
 Proof.
-  intros ? ?. rewrite -wp_bin_op //; [].
+  intros. rewrite -wp_bin_op //; [].
   destruct (bool_decide_reflect (n1 ≤ n2)); by eauto with omega.
 Qed.
 
@@ -109,7 +84,7 @@ Lemma wp_lt E (n1 n2 : nat) P Q :
   (n1 ≥ n2 → P ⊑ ▷ Q (LitV false)) →
   P ⊑ wp E (BinOp LtOp (Lit n1) (Lit n2)) Q.
 Proof.
-  intros ? ?. rewrite -wp_bin_op //; [].
+  intros. rewrite -wp_bin_op //; [].
   destruct (bool_decide_reflect (n1 < n2)); by eauto with omega.
 Qed.
 
@@ -118,7 +93,7 @@ Lemma wp_eq E (n1 n2 : nat) P Q :
   (n1 ≠ n2 → P ⊑ ▷ Q (LitV false)) →
   P ⊑ wp E (BinOp EqOp (Lit n1) (Lit n2)) Q.
 Proof.
-  intros ? ?. rewrite -wp_bin_op //; [].
+  intros. rewrite -wp_bin_op //; [].
   destruct (bool_decide_reflect (n1 = n2)); by eauto with omega.
 Qed.
 
