heap_lang/tests.v
@@ -7,12 +7,18 @@ Module LangTests.
   Definition add := (Lit 21 + Lit 21)%L.
   Goal ∀ σ, prim_step add σ (Lit 42) σ None.
   Proof. intros; do_step done. Qed.
-  Definition rec_app : expr := (rec:: #0 #1) (Lit 0).
+  Definition rec_app : expr := (rec: "f" "x" := "f" "x") (Lit 0).
   Goal ∀ σ, prim_step rec_app σ rec_app σ None.
-  Proof. intros; do_step done. Qed.
-  Definition lam : expr := λ: #0 + Lit 21.
+  Proof.
+    intros. rewrite /rec_app. (* FIXME: do_step does not work here *)
+    by eapply (Ectx_step  _ _ _ _ _ []), (BetaS _ _ _ _ (LitV (LitNat 0))).
+  Qed.
+  Definition lam : expr := λ: "x", "x" + Lit 21.
   Goal ∀ σ, prim_step (lam (Lit 21)) σ add σ None.
-  Proof. rewrite /lam /Lam. intros; do_step done. Qed.
+  Proof.
+    intros. rewrite /lam. (* FIXME: do_step does not work here *)
+    by eapply (Ectx_step  _ _ _ _ _ []), (BetaS "" "x" ("x" + Lit 21) _ (LitV 21)).
+  Qed.
 End LangTests.
 
 Module LiftingTests.
@@ -20,22 +26,23 @@ Module LiftingTests.
   Implicit Types P : iProp heap_lang Σ.
   Implicit Types Q : val → iProp heap_lang Σ.
 
-  Definition e  : expr := let: ref (Lit 1) in #0 <- !#0 + Lit 1; !#0.
-  Goal ∀ σ E, (ownP σ : iProp heap_lang Σ) ⊑ (wp E e (λ v, ■(v = LitV 2))).
+  Definition e  : expr :=
+    let: "x" := ref (Lit 1) in "x" <- !"x" + Lit 1; !"x".
+  Goal ∀ σ E, (ownP σ : iProp heap_lang Σ) ⊑ (wp E e (λ v, ■ (v = LitV 2))).
   Proof.
     move=> σ E. rewrite /e.
-    rewrite -wp_let. rewrite -wp_alloc_pst; last done.
+    rewrite -wp_let /= -wp_alloc_pst //=.
     apply sep_intro_True_r; first done.
-    rewrite -later_intro. apply forall_intro=>l.
-    apply wand_intro_l. rewrite right_id. apply const_elim_l; move=>_.
-    rewrite -later_intro. asimpl.
-    rewrite -(wp_bindi (SeqCtx (Load (Loc _)))).
+    rewrite -later_intro; apply forall_intro=>l; apply wand_intro_l.
+    rewrite right_id; apply const_elim_l=> _.
+    rewrite -later_intro.
+    rewrite -(wp_bindi (SeqCtx (Load (Loc _)))) /=.
     (* FIXME: doing simpl here kills the Seq, turns it all the way into Rec *)
-    rewrite -(wp_bindi (StoreRCtx (LocV _))).
-    rewrite -(wp_bindi (BinOpLCtx PlusOp _)).
+    rewrite -(wp_bindi (StoreRCtx (LocV _))) /=.
+    rewrite -(wp_bindi (BinOpLCtx PlusOp _)) /=.
     rewrite -wp_load_pst; first (apply sep_intro_True_r; first done); last first.
     { by rewrite lookup_insert. } (* RJ FIXME: figure out why apply and eapply fail. *)
-    rewrite -later_intro. apply wand_intro_l. rewrite right_id.
+    rewrite -later_intro; apply wand_intro_l; rewrite right_id.
     rewrite -wp_bin_op // -later_intro.
     rewrite -wp_store_pst; first (apply sep_intro_True_r; first done); last first.
     { by rewrite lookup_insert. }
@@ -49,56 +56,50 @@ Module LiftingTests.
   Qed.
 
   Definition FindPred (n2 : expr) : expr :=
-    rec:: let: #1 + Lit 1 in if #0 < n2.[ren(+3)] then #1 #0 else #2.
+    rec: "pred" "y" :=
+      let: "yp" := "y" + Lit 1 in
+      if "yp" < n2 then "pred" "yp" else "y".
   Definition Pred : expr :=
-    λ: if #0 ≤ Lit 0 then Lit 0 else FindPred #0 (Lit 0).
+    λ: "x", if "x" ≤ Lit 0 then Lit 0 else FindPred "x" (Lit 0).
 
   Lemma FindPred_spec n1 n2 E Q :
-    (■ (n1 < n2) ∧ Q (LitV $ pred n2)) ⊑ wp E (FindPred (Lit n2) (Lit n1)) Q.
+    (■ (n1 < n2) ∧ Q (LitV (pred n2))) ⊑ wp E (FindPred (Lit n2) (Lit n1)) Q.
   Proof.
     revert n1. apply löb_all_1=>n1.
-    rewrite -wp_rec //. asimpl.
-    (* Get rid of the ▷ in the premise. *)
-    etransitivity; first (etransitivity; last eapply equiv_spec, later_and).
-    { apply and_mono; first done. by rewrite -later_intro. }
-    apply later_mono.
+    rewrite (commutative uPred_and (■ _)%I) associative; apply const_elim_r=>?.
+    rewrite -wp_rec //=.
+    (* FIXME: ssr rewrite fails with "Error: _pattern_value_ is used in conclusion." *)
+    rewrite ->(later_intro (Q _)).
+    rewrite -!later_and; apply later_mono.
     (* Go on *)
-    rewrite -wp_let.
-    rewrite -wp_bin_op //. asimpl.
-    rewrite -(wp_bindi (IfCtx _ _)).
-    rewrite -!later_intro /=.
-    apply wp_lt; intros Hn12.
-    * rewrite -wp_if_true.
-      rewrite -!later_intro. asimpl.
-      rewrite (forall_elim (S n1)).
-      eapply impl_elim; first by eapply and_elim_l. apply and_intro.
-      + apply const_intro; omega.
-      + by rewrite !and_elim_r.
-    * rewrite -wp_if_false.
-      rewrite -!later_intro -wp_value' //.
-      rewrite and_elim_r. apply const_elim_l=>Hle.
-      by replace n1 with (pred n2) by omega.
+    rewrite -wp_let -wp_bin_op //= -(wp_bindi (IfCtx _ _)) /= -!later_intro.
+    apply wp_lt=> ?.
+    - rewrite -wp_if_true.
+      rewrite -!later_intro (forall_elim (n1 + 1)) const_equiv; last omega.
+      by rewrite left_id impl_elim_l.
+    - assert (n1 = pred n2) as -> by omega.
+      rewrite -wp_if_false.
+      by rewrite -!later_intro -wp_value' // and_elim_r.
   Qed.
 
-  Lemma Pred_spec n E Q :
-    ▷Q (LitV $ pred n) ⊑ wp E (Pred $ Lit n) Q.
+  Lemma Pred_spec n E Q : ▷ Q (LitV (pred n)) ⊑ wp E (Pred (Lit n)) Q.
   Proof.
-    rewrite -wp_lam //. asimpl.
+    rewrite -wp_lam //=.
     rewrite -(wp_bindi (IfCtx _ _)).
     apply later_mono, wp_le=> Hn.
     - rewrite -wp_if_true.
-      rewrite -!later_intro -wp_value' //.
-      by replace n with 0 by omega.
+      rewrite -!later_intro -wp_value' //=.
+      auto with f_equal omega.
     - rewrite -wp_if_false.
       rewrite -!later_intro -FindPred_spec.
       auto using and_intro, const_intro with omega.
   Qed.
 
   Goal ∀ E,
-    True ⊑ wp (Σ:=Σ) E (let: Pred $ Lit 42 in Pred #0) (λ v, ■(v = LitV 40)).
+    True ⊑ wp (Σ:=Σ) E (let: "x" := Pred (Lit 42) in Pred "x")
+                       (λ v, ■ (v = LitV 40)).
   Proof.
-    intros E. rewrite -wp_let. rewrite -Pred_spec -!later_intro.
-    asimpl. (* TODO RJ: Can we somehow make it so that Pred gets folded again? *)
+    intros E. rewrite -wp_let. rewrite -Pred_spec -!later_intro /=.
     rewrite -Pred_spec -later_intro. by apply const_intro.
   Qed.
 End LiftingTests.
